theories/CodegenWasm/LambdaANF_to_Wasm_primitives.v
@@ -3,8 +3,8 @@ From CertiCoq Require Import LambdaANF.toplevel LambdaANF.cps_util.
 
 From CertiCoq Require Import Common.Common Common.compM Common.Pipeline_utils.
 Require Import ExtLib.Structures.Monad.
-From MetaCoq.Utils Require Import bytestring MCString.
-From Coq Require Import ZArith BinNat List Lia.
+From MetaCoq Require Import Common.Kernames Utils.bytestring Utils.MCString.
+From Coq Require Import ZArith BinNat List Lia Uint63.
 
 Require Import MSets.MSetAVL.
 From Coq Require Import FMapAVL.
@@ -13,11 +13,14 @@ Require Import POrderedType.
 Require Import LambdaANF.cps LambdaANF.cps_show.
 Import MonadNotation.
 
-Definition nat_to_i32val n :=
-  VAL_int32 (Wasm_int.Int32.repr (BinInt.Z.of_nat n)).
 
-Definition nat_to_i64val n :=
-  VAL_int64 (Wasm_int.Int64.repr (BinInt.Z.of_nat n)).
+Import SigTNotations.
+
+Notation int63 := Uint63.int.
+
+(* Notation "k1 =? k2" := (Kername.eqb k1 k2). *)
+
+Notation "( 'primInt' x )" := (AstCommon.primInt ; x).
 
 (* **** TRANSLATE PRIMITIVE VALUES **** *)
 
@@ -29,37 +32,73 @@ Definition translate_primitive_value (p : AstCommon.primitive) : error Wasm_int.
   
 (* **** TRANSLATE PRIMITIVE OPERATIONS **** *)
 
-Section PrimitiveOperators.
-
-Variables global_mem_ptr glob_tmp1 glob_tmp2 glob_tmp3 glob_tmp4 : globalidx.
-
 Definition primInt63ModPath : Kernames.modpath :=
   Kernames.MPfile [ "PrimInt63"%bs ; "Int63"%bs ; "Cyclic"%bs ; "Numbers"%bs ; "Coq"%bs ].
 
-Definition primInt63Add        : Kernames.kername := (primInt63ModPath, "add"%bs).
-Definition primInt63Addc       : Kernames.kername := (primInt63ModPath, "addc"%bs).
-Definition primInt63Addcarryc  : Kernames.kername := (primInt63ModPath, "addcarryc"%bs).
-Definition primInt63Sub        : Kernames.kername := (primInt63ModPath, "sub"%bs).
-Definition primInt63Subc       : Kernames.kername := (primInt63ModPath, "subc"%bs).
-Definition primInt63Subcarryc  : Kernames.kername := (primInt63ModPath, "subcarryc"%bs).
-Definition primInt63Mul        : Kernames.kername := (primInt63ModPath, "mul"%bs).
-Definition primInt63Mulc       : Kernames.kername := (primInt63ModPath, "mulc"%bs).
-Definition primInt63Div        : Kernames.kername := (primInt63ModPath, "div"%bs).
-Definition primInt63Mod        : Kernames.kername := (primInt63ModPath, "mod"%bs).
-Definition primInt63Land       : Kernames.kername := (primInt63ModPath, "land"%bs).
-Definition primInt63Lor        : Kernames.kername := (primInt63ModPath, "lor"%bs).
-Definition primInt63Lxor       : Kernames.kername := (primInt63ModPath, "lxor"%bs).
-Definition primInt63Lsl        : Kernames.kername := (primInt63ModPath, "lsl"%bs).
-Definition primInt63Lsr        : Kernames.kername := (primInt63ModPath, "lsr"%bs).
-Definition primInt63Compare    : Kernames.kername := (primInt63ModPath, "compare"%bs).
-Definition primInt63Eqb        : Kernames.kername := (primInt63ModPath, "eqb"%bs).
-Definition primInt63Ltb        : Kernames.kername := (primInt63ModPath, "ltb"%bs).
-Definition primInt63Leb        : Kernames.kername := (primInt63ModPath, "leb"%bs).
-Definition primInt63Head0      : Kernames.kername := (primInt63ModPath, "head0"%bs).
-Definition primInt63Tail0      : Kernames.kername := (primInt63ModPath, "tail0"%bs).
-Definition primInt63Addmuldiv  : Kernames.kername := (primInt63ModPath, "addmuldiv"%bs).
-Definition primInt63Diveucl    : Kernames.kername := (primInt63ModPath, "diveucl"%bs).
-Definition primInt63Diveucl_21 : Kernames.kername := (primInt63ModPath, "diveucl_21"%bs).
+Inductive primop :=
+| PrimInt63add
+| PrimInt63sub
+| PrimInt63mul
+| PrimInt63div
+| PrimInt63mod
+| PrimInt63lsl
+| PrimInt63lsr
+| PrimInt63land
+| PrimInt63lor
+| PrimInt63lxor
+| PrimInt63eqb
+| PrimInt63ltb
+| PrimInt63leb
+| PrimInt63compare
+| PrimInt63addc
+| PrimInt63addcarryc
+| PrimInt63subc
+| PrimInt63subcarryc
+| PrimInt63mulc
+| PrimInt63head0
+| PrimInt63tail0
+| PrimInt63diveucl
+| PrimInt63diveucl_21
+| PrimInt63addmuldiv.
+
+Definition primop_map : KernameMap.t primop :=
+  KernameMap.add (primInt63ModPath, "add") PrimInt63add
+    (KernameMap.add (primInt63ModPath, "sub") PrimInt63sub
+    (KernameMap.add (primInt63ModPath, "mul") PrimInt63mul
+    (KernameMap.add (primInt63ModPath, "div") PrimInt63div
+    (KernameMap.add (primInt63ModPath, "mod") PrimInt63mod
+    (KernameMap.add (primInt63ModPath, "lsl") PrimInt63lsl
+    (KernameMap.add (primInt63ModPath, "lsr") PrimInt63lsr
+    (KernameMap.add (primInt63ModPath, "land") PrimInt63land
+    (KernameMap.add (primInt63ModPath, "lor") PrimInt63lor
+    (KernameMap.add (primInt63ModPath, "lxor") PrimInt63lxor
+    (KernameMap.add (primInt63ModPath, "eqb") PrimInt63eqb
+    (KernameMap.add (primInt63ModPath, "ltb") PrimInt63ltb
+    (KernameMap.add (primInt63ModPath, "leb") PrimInt63leb
+    (KernameMap.add (primInt63ModPath, "compare") PrimInt63compare
+    (KernameMap.add (primInt63ModPath, "addc") PrimInt63addc
+    (KernameMap.add (primInt63ModPath, "addcarryc") PrimInt63addcarryc
+    (KernameMap.add (primInt63ModPath, "subc") PrimInt63subc
+    (KernameMap.add (primInt63ModPath, "subcarryc") PrimInt63subcarryc
+    (KernameMap.add (primInt63ModPath, "mulc") PrimInt63mulc
+    (KernameMap.add (primInt63ModPath, "head0") PrimInt63head0
+    (KernameMap.add (primInt63ModPath, "tail0") PrimInt63tail0
+    (KernameMap.add (primInt63ModPath, "diveucl") PrimInt63diveucl
+    (KernameMap.add (primInt63ModPath, "diveucl_21") PrimInt63diveucl_21
+    (KernameMap.add (primInt63ModPath, "addmuldiv") PrimInt63addmuldiv
+    (KernameMap.empty primop)))))))))))))))))))))))).
+
+Section Primitives.
+
+Variables global_mem_ptr glob_tmp1 glob_tmp2 glob_tmp3 glob_tmp4 : globalidx.
+
+Variables true_tag false_tag eq_tag lt_tag gt_tag c0_tag c1_tag pair_tag : ctor_tag.
+
+Definition nat_to_i32val n :=
+  VAL_int32 (Wasm_int.Int32.repr (BinInt.Z.of_nat n)).
+
+Definition nat_to_i64val n :=
+  VAL_int64 (Wasm_int.Int64.repr (BinInt.Z.of_nat n)).
 
 Definition maxuint31 := VAL_int64 (Wasm_int.Int64.repr 2147483647%Z).
 Definition maxuint63 := VAL_int64 (Wasm_int.Int64.repr 9223372036854775807%Z).
@@ -74,11 +113,12 @@ Definition increment_global_mem_ptr i :=
   ; BI_global_set global_mem_ptr
   ].
 
-Definition apply_binop_and_store_i64 (op : list basic_instruction) x y :=
+Definition apply_binop_and_store_i64 (op : binop_i) (x y : localidx) (mask : bool) : list basic_instruction :=
   BI_global_get global_mem_ptr :: (* Address to store the result of the operation *)
   load_local_i64 x ++             (* Load the arguments onto the stack *)
   load_local_i64 y ++
-  op ++
+  [ BI_binop T_i64 (Binop_i op) ] ++
+  (if mask then [ BI_const_num maxuint63 ; BI_binop T_i64 (Binop_i BOI_and) ] else []) ++ 
   [ BI_store T_i64 None 2%N 0%N   (* Store the result *)
   ; BI_global_get global_mem_ptr  (* Put the address where the result was stored on the stack *)
   ] ++
@@ -89,15 +129,9 @@ Definition make_carry (ord : nat) (gidx : globalidx) : list basic_instruction:=
   ; BI_global_get gidx
   ; BI_store T_i64 None 2%N 0%N
   ; BI_global_get global_mem_ptr
-  (* ; BI_const_num (nat_to_i32val 8) *)
-  (* ; BI_binop T_i32 (Binop_i BOI_add) *)
-  (* ; BI_global_set constr_alloc_ptr *)
-  (* ; BI_global_get constr_alloc_ptr *)
   ; BI_const_num (nat_to_i32val ord)
   ; BI_store T_i32 None 2%N 8%N
   ; BI_global_get global_mem_ptr
-  (* ; BI_const_num (nat_to_i32val 12) *)
-  (* ; BI_binop T_i32 (Binop_i BOI_add) *)
   ; BI_global_get global_mem_ptr
   ; BI_store T_i32 None 2%N 12%N
   ; BI_global_get global_mem_ptr
@@ -105,19 +139,36 @@ Definition make_carry (ord : nat) (gidx : globalidx) : list basic_instruction:=
   ; BI_binop T_i32 (Binop_i BOI_add)
   ] ++ increment_global_mem_ptr 16.
 
-
-Definition apply_carry_operation x y  (ord1 ord2 : nat) (ops relops : list basic_instruction) : list basic_instruction :=
-    load_local_i64 x ++
-    load_local_i64 y ++
-    ops ++
+Definition apply_exact_add_operation (x y : localidx) (addone : bool) : list basic_instruction :=
+    load_local_i64 x ++ load_local_i64 y ++
+    [ BI_binop T_i64 (Binop_i BOI_add) ] ++ 
+    (if addone then 
+       [ BI_const_num (nat_to_i64val 1) ; BI_binop T_i64 (Binop_i BOI_add) ] 
+     else []) ++
     [ BI_const_num maxuint63
     ; BI_binop T_i64 (Binop_i BOI_and)
     ; BI_global_set glob_tmp1
-    ] ++
-    relops ++
-    [ BI_if (BT_valtype (Some (T_num T_i32)))
-        (make_carry ord1 glob_tmp1)
-        (make_carry ord2 glob_tmp1)
+    ; BI_global_get glob_tmp1
+    ] ++ 
+    load_local_i64 x ++
+    [ BI_relop T_i64 (Relop_i ((if addone then ROI_le else ROI_lt) SX_U)) 
+    ; BI_if (BT_valtype (Some (T_num T_i32))) (make_carry 1 glob_tmp1) (make_carry 0 glob_tmp1) 
+    ].
+
+Definition apply_exact_sub_operation (x y : localidx) (subone : bool) : list basic_instruction :=
+    load_local_i64 x ++ load_local_i64 y ++
+    [ BI_binop T_i64 (Binop_i BOI_sub) ] ++
+    (if subone then 
+       [ BI_const_num (nat_to_i64val 1) ; BI_binop T_i64 (Binop_i BOI_sub) ] 
+     else []) ++
+    [ BI_const_num maxuint63
+    ; BI_binop T_i64 (Binop_i BOI_and)
+    ; BI_global_set glob_tmp1
+    ] ++ 
+    load_local_i64 y ++
+    load_local_i64 x ++
+    [ BI_relop T_i64 (Relop_i ((if subone then ROI_lt else ROI_le) SX_U))
+    ; BI_if (BT_valtype (Some (T_num T_i32))) (make_carry 0 glob_tmp1) (make_carry 1 glob_tmp1) 
     ].
 
 (* Assumptions for constructing a prod value:
@@ -127,39 +178,23 @@ Definition make_product (gidx1 gidx2 : N) : list basic_instruction :=
   [ BI_global_get global_mem_ptr
   ; BI_global_get gidx1
   ; BI_store T_i64 None 2%N 0%N
-  (* ; BI_global_get global_mem_ptr *)
-  (* ; BI_const_num (nat_to_i32val 8) *)
-  (* ; BI_binop T_i32 (Binop_i BOI_add) *)
   ; BI_global_get global_mem_ptr
   ; BI_global_get gidx2
   ; BI_store T_i64 None 2%N 8%N
-  (* ; BI_global_get global_mem_ptr *)
-  (* ; BI_const_num (nat_to_i32val 16) *)
-  (* ; BI_binop T_i32 (Binop_i BOI_add) *)
-  (* ; BI_global_set constr_alloc_ptr *)
   ; BI_global_get global_mem_ptr
   ; BI_const_num (nat_to_i32val 0)
   ; BI_store T_i32 None 2%N 16%N
-
-  (* ; BI_global_get global_mem_ptr *)
-  (* ; BI_const_num (nat_to_i32val 20) *)
-  (* ; BI_binop T_i32 (Binop_i BOI_add) *)
   ; BI_global_get global_mem_ptr
   ; BI_global_get global_mem_ptr
   ; BI_store T_i32 None 2%N 20%N
-
   ; BI_global_get global_mem_ptr
-  (* ; BI_const_num (nat_to_i32val 24) *)
-  (* ; BI_binop T_i32 (Binop_i BOI_add) *)
   ; BI_global_get global_mem_ptr
   ; BI_const_num (nat_to_i32val 8)
   ; BI_binop T_i32 (Binop_i BOI_add)
   ; BI_store T_i32 None 2%N 24%N
-
   ; BI_global_get global_mem_ptr
   ; BI_const_num (nat_to_i32val 16)
   ; BI_binop T_i32 (Binop_i BOI_add)
-  (* ; BI_global_get constr_alloc_ptr *)
   ] ++ increment_global_mem_ptr 28.
 
 (* Assumptions about constructor environment for primitive operations that return bools:
@@ -174,350 +209,308 @@ Definition make_boolean_valued_comparison x y relop : list basic_instruction :=
       [ BI_const_num (nat_to_i32val 3) ] (* 2 * ordinal(false) + 1 *)
   ].
 
-Definition translate_primitive_binary_op op_name x y : error (list basic_instruction) :=
-  if Kername.eqb op_name primInt63Add then
-    Ret (apply_binop_and_store_i64 [ BI_binop T_i64 (Binop_i BOI_add) ; BI_const_num maxuint63 ; BI_binop T_i64 (Binop_i BOI_and) ] x y)
-  else if Kername.eqb op_name primInt63Sub then
-    Ret (apply_binop_and_store_i64 [ BI_binop T_i64 (Binop_i BOI_sub) ; BI_const_num maxuint63 ; BI_binop T_i64 (Binop_i BOI_and) ] x y)
-  else if Kername.eqb op_name primInt63Mul then
-    Ret (apply_binop_and_store_i64 [ BI_binop T_i64 (Binop_i BOI_mul) ; BI_const_num maxuint63 ; BI_binop T_i64 (Binop_i BOI_and) ] x y)
-  else if Kername.eqb op_name primInt63Div then
-    Ret (BI_global_get global_mem_ptr ::
-         load_local_i64 y ++
-         [ BI_testop T_i64 TO_eqz
-         ; BI_if (BT_valtype (Some (T_num T_i64)))
-             [ BI_const_num (nat_to_i64val 0) ]
-             (load_local_i64 x ++ load_local_i64 y ++ [ BI_binop T_i64 (Binop_i (BOI_div SX_U)) ])
-         ; BI_store T_i64 None 2%N 0%N
-         ; BI_global_get global_mem_ptr
-         ] ++ increment_global_mem_ptr 8)
-  else if Kername.eqb op_name primInt63Mod then
-    Ret(BI_global_get global_mem_ptr ::
-        load_local_i64 y ++
-        [ BI_testop T_i64 TO_eqz
-        ; BI_if (BT_valtype (Some (T_num T_i64)))
-            (load_local_i64 x)
-            (load_local_i64 x ++ load_local_i64 y ++ [ BI_binop T_i64 (Binop_i (BOI_rem SX_U)) ])
-        ; BI_store T_i64 None 2%N 0%N
-        ; BI_global_get global_mem_ptr
-        ] ++ increment_global_mem_ptr 8)
-  else if Kername.eqb op_name primInt63Land then
-    Ret (apply_binop_and_store_i64 [ BI_binop T_i64 (Binop_i BOI_and) ] x y)
-  else if Kername.eqb op_name primInt63Lor then
-    Ret (apply_binop_and_store_i64 [ BI_binop T_i64 (Binop_i BOI_or) ] x y)
-  else if Kername.eqb op_name primInt63Lxor then
-    Ret (apply_binop_and_store_i64 [ BI_binop T_i64 (Binop_i BOI_xor) ] x y)
-  else if Kername.eqb op_name primInt63Lsl then
-    Ret (BI_global_get global_mem_ptr ::
-         load_local_i64 y ++
-         [ BI_const_num (nat_to_i64val 63)
-         ; BI_relop T_i64 (Relop_i (ROI_lt SX_U))
-         ; BI_if (BT_valtype (Some (T_num T_i64)))
-             (load_local_i64 x ++
-              load_local_i64 y ++
-              [ BI_binop T_i64 (Binop_i BOI_shl) ; BI_const_num maxuint63 ; BI_binop T_i64 (Binop_i BOI_and) ])
-             [ BI_const_num (nat_to_i64val 0) ]
-         ; BI_store T_i64 None 2%N 0%N
-         ; BI_global_get global_mem_ptr
-         ] ++ increment_global_mem_ptr 8)
 
-  else if Kername.eqb op_name primInt63Lsr then
-    Ret (BI_global_get global_mem_ptr ::
-         load_local_i64 y ++
-         [ BI_const_num (nat_to_i64val 63)
-         ; BI_relop T_i64 (Relop_i (ROI_lt SX_U))
-         ; BI_if (BT_valtype (Some (T_num T_i64)))
-             (load_local_i64 x ++ load_local_i64 y ++ [ BI_binop T_i64 (Binop_i (BOI_shr SX_U)) ])
-             [ BI_const_num (nat_to_i64val 0) ]
-         ; BI_store T_i64 None 2%N 0%N
-         ; BI_global_get global_mem_ptr
-         ] ++ increment_global_mem_ptr 8)
+Definition compare_instrs x y : list basic_instruction :=
+  [ BI_local_get x
+    ; BI_load T_i64 None 2%N 0%N
+    ; BI_local_get y
+    ; BI_load T_i64 None 2%N 0%N
+    ; BI_relop T_i64 (Relop_i (ROI_lt SX_U))
+    ; BI_if (BT_valtype (Some (T_num T_i32)))
+        [ BI_const_num (nat_to_i32val 3) ] (* 2 * ordinal(Lt) + 1 *)
+        (load_local_i64 x ++
+           load_local_i64 y ++
+           [ BI_relop T_i64 (Relop_i ROI_eq)
+             ; BI_if (BT_valtype (Some (T_num T_i32)))
+                 [ BI_const_num (nat_to_i32val 1) ] (* 2 * ordinal(Eq) + 1 *)
+                 [ BI_const_num (nat_to_i32val 5) ] (* 2 * ordinal(Gt) + 1*)
+           ])
+  ].
 
-  else if Kername.eqb op_name primInt63Eqb then
-    Ret (make_boolean_valued_comparison x y ROI_eq)
+Definition div_instrs (x y : localidx) : list basic_instruction :=
+  BI_global_get global_mem_ptr ::
+    load_local_i64 y ++
+    [ BI_testop T_i64 TO_eqz
+    ; BI_if (BT_valtype (Some (T_num T_i64)))
+        [ BI_const_num (nat_to_i64val 0) ]
+        (load_local_i64 x ++ load_local_i64 y ++ [ BI_binop T_i64 (Binop_i (BOI_div SX_U)) ])
+    ; BI_store T_i64 None 2%N 0%N
+    ; BI_global_get global_mem_ptr
+    ] ++ increment_global_mem_ptr 8.
 
-  else if Kername.eqb op_name primInt63Ltb then
-    Ret (make_boolean_valued_comparison x y (ROI_lt SX_U))
 
-  else if Kername.eqb op_name primInt63Leb then
-    Ret (make_boolean_valued_comparison x y (ROI_le SX_U))
+Definition mod_instrs (x y : localidx) : list basic_instruction :=
+  BI_global_get global_mem_ptr ::
+    load_local_i64 y ++
+    [ BI_testop T_i64 TO_eqz
+    ; BI_if (BT_valtype (Some (T_num T_i64)))
+        (load_local_i64 x)
+        (load_local_i64 x ++ load_local_i64 y ++ [ BI_binop T_i64 (Binop_i (BOI_rem SX_U)) ])
+    ; BI_store T_i64 None 2%N 0%N
+    ; BI_global_get global_mem_ptr
+    ] ++ increment_global_mem_ptr 8.
 
-  (* Assumptions about constructor environment for compare:
-       1. ordinal(Eq) = 0
-       2. ordinal(Lt) = 1
-       3. ordinal(Gt) = 2 *)
-  else if Kername.eqb op_name primInt63Compare then
-    Ret ([ BI_local_get x
-         ; BI_load T_i64 None 2%N 0%N
-         ; BI_local_get y
-         ; BI_load T_i64 None 2%N 0%N
-         ; BI_relop T_i64 (Relop_i (ROI_lt SX_U))
-         ; BI_if (BT_valtype (Some (T_num T_i32)))
-             [ BI_const_num (nat_to_i32val 3) ] (* 2 * ordinal(Lt) + 1 *)
-             (load_local_i64 x ++
-              load_local_i64 y ++
-              [ BI_relop T_i64 (Relop_i ROI_eq)
-              ; BI_if (BT_valtype (Some (T_num T_i32)))
-                  [ BI_const_num (nat_to_i32val 1) ] (* 2 * ordinal(Eq) + 1 *)
-                  [ BI_const_num (nat_to_i32val 5) ] (* 2 * ordinal(Gt) + 1*)
-              ])
-         ])
+Definition shift_instrs (x y : localidx) shiftop (mask : bool) : list basic_instruction :=
+  BI_global_get global_mem_ptr ::
+    load_local_i64 y ++
+    [ BI_const_num (nat_to_i64val 63)
+    ; BI_relop T_i64 (Relop_i (ROI_lt SX_U))
+    ; BI_if (BT_valtype (Some (T_num T_i64)))
+        (load_local_i64 x ++ 
+           load_local_i64 y ++ 
+           BI_binop T_i64 (Binop_i shiftop) ::
+           (if mask then [ BI_const_num maxuint63 ; BI_binop T_i64 (Binop_i BOI_and) ] else []))
+        [ BI_const_num (nat_to_i64val 0) ]
+    ; BI_store T_i64 None 2%N 0%N
+    ; BI_global_get global_mem_ptr
+    ] ++ increment_global_mem_ptr 8.
 
-       (* Assumptions for constructing a carry value:
-          - The argument is stored in global with index gidx
-          - ordinal(C0) = 0
-          - ordinal(C1) = 1 *)
-  else if Kername.eqb op_name primInt63Addc then
-    Ret (apply_carry_operation x y 1 0
-           [ BI_binop T_i64 (Binop_i BOI_add) ]
-           ([ BI_global_get glob_tmp1 ] ++
-              load_local_i64 x ++
-              [ BI_relop T_i64 (Relop_i (ROI_lt SX_U))]))
-
-  else if Kername.eqb op_name primInt63Addcarryc then
-    Ret (apply_carry_operation x y 1 0
-           [ BI_binop T_i64 (Binop_i BOI_add)
-             ; BI_const_num (nat_to_i64val 1)
-             ; BI_binop T_i64 (Binop_i BOI_add) ]
-           ([ BI_global_get glob_tmp1 ] ++
-              load_local_i64 x ++
-              [ BI_relop T_i64 (Relop_i (ROI_le SX_U))]))
-
-  else if Kername.eqb op_name primInt63Subc then
-    Ret (apply_carry_operation x y 0 1
-           [ BI_binop T_i64 (Binop_i BOI_sub) ]
-           (load_local_i64 y ++
-              load_local_i64 x ++
-              [ BI_relop T_i64 (Relop_i (ROI_le SX_U))]))
-
-  else if Kername.eqb op_name primInt63Subcarryc then
-    Ret (apply_carry_operation x y 0 1
-           [ BI_binop T_i64 (Binop_i BOI_sub)
-           ; BI_const_num (nat_to_i64val 1)
-           ; BI_binop T_i64 (Binop_i BOI_sub) ]
-           (load_local_i64 y ++
-              load_local_i64 x ++
-              [ BI_relop T_i64 (Relop_i (ROI_lt SX_U))]))
-
-  else if Kername.eqb op_name primInt63Mulc then
-    Ret (load_local_i64 x ++
-         [ BI_const_num (nat_to_i64val 62) ; BI_binop T_i64 (Binop_i (BOI_shr SX_U)) ; BI_testop T_i64 TO_eqz ] ++
-         load_local_i64 y ++
-         [ BI_const_num (nat_to_i64val 62) ; BI_binop T_i64 (Binop_i (BOI_shr SX_U)) ; BI_testop T_i64 TO_eqz ] ++
-         [ BI_binop T_i32 (Binop_i BOI_or)
-         ; BI_if (BT_valtype None)
-             (load_local_i64 y ++ [ BI_global_set glob_tmp3 ])
-             (load_local_i64 y ++
-              [ BI_const_num (VAL_int64 (Wasm_int.Int64.repr 4611686018427387904%Z))
-              ; BI_binop T_i64 (Binop_i BOI_xor)
-              ; BI_global_set glob_tmp3
-              ])
-         ] ++
-         (* glob_tmp1 <- let hx = x >> 31 *)
-         load_local_i64 x ++
-         [ BI_const_num (nat_to_i64val 31) ; BI_binop T_i64 (Binop_i (BOI_shr SX_U)) ; BI_global_set glob_tmp1 ] ++
-         (* glob_tmp2 <- let lx = x & ((1 << 31) - 1) *)
-         load_local_i64 x ++
-         [ BI_const_num maxuint31 ; BI_binop T_i64 (Binop_i BOI_and) ; BI_global_set glob_tmp2 ] ++
-         (* glob_tmp4 <- let hy =  y >> 31 *)
-         [ BI_global_get glob_tmp3 ; BI_const_num (nat_to_i64val 31) ; BI_binop T_i64 (Binop_i (BOI_shr SX_U)) ; BI_global_set glob_tmp4 ] ++
-         (* glob_tmp3 <- let ly = y & ((1 << 31) - 1) *)
-         [ BI_global_get glob_tmp3 ; BI_const_num maxuint31 ; BI_binop T_i64 (Binop_i BOI_and) ; BI_global_set glob_tmp3 ] ++
-         [ BI_global_get glob_tmp1 ; BI_global_get glob_tmp4 ; BI_binop T_i64 (Binop_i BOI_mul) ] ++
-         [ BI_global_get glob_tmp1 ; BI_global_get glob_tmp3 ; BI_binop T_i64 (Binop_i BOI_mul) ] ++
-         [ BI_global_get glob_tmp2 ; BI_global_get glob_tmp4 ; BI_binop T_i64 (Binop_i BOI_mul) ] ++
-         [ BI_global_get glob_tmp2 ; BI_global_get glob_tmp3 ; BI_binop T_i64 (Binop_i BOI_mul) ] ++
-         (* glob_tmp4 <- let lxy = lx * ly
+Definition mulc_instrs (x y : localidx) : list basic_instruction :=
+  load_local_i64 x ++
+    [ BI_const_num (nat_to_i64val 62) ; BI_binop T_i64 (Binop_i (BOI_shr SX_U)) ; BI_testop T_i64 TO_eqz ] ++
+    load_local_i64 y ++
+    [ BI_const_num (nat_to_i64val 62) ; BI_binop T_i64 (Binop_i (BOI_shr SX_U)) ; BI_testop T_i64 TO_eqz ] ++
+    [ BI_binop T_i32 (Binop_i BOI_or)
+      ; BI_if (BT_valtype None)
+          (load_local_i64 y ++ [ BI_global_set glob_tmp3 ])
+          (load_local_i64 y ++
+             [ BI_const_num (VAL_int64 (Wasm_int.Int64.repr 4611686018427387904%Z))
+               ; BI_binop T_i64 (Binop_i BOI_xor)
+               ; BI_global_set glob_tmp3
+          ])
+    ] ++
+    (* glob_tmp1 <- let hx = x >> 31 *)
+    load_local_i64 x ++
+    [ BI_const_num (nat_to_i64val 31) ; BI_binop T_i64 (Binop_i (BOI_shr SX_U)) ; BI_global_set glob_tmp1 ] ++
+    (* glob_tmp2 <- let lx = x & ((1 << 31) - 1) *)
+    load_local_i64 x ++
+    [ BI_const_num maxuint31 ; BI_binop T_i64 (Binop_i BOI_and) ; BI_global_set glob_tmp2 ] ++
+    (* glob_tmp4 <- let hy =  y >> 31 *)
+    [ BI_global_get glob_tmp3 ; BI_const_num (nat_to_i64val 31) ; BI_binop T_i64 (Binop_i (BOI_shr SX_U)) ; BI_global_set glob_tmp4 ] ++
+    (* glob_tmp3 <- let ly = y & ((1 << 31) - 1) *)
+    [ BI_global_get glob_tmp3 ; BI_const_num maxuint31 ; BI_binop T_i64 (Binop_i BOI_and) ; BI_global_set glob_tmp3 ] ++
+    [ BI_global_get glob_tmp1 ; BI_global_get glob_tmp4 ; BI_binop T_i64 (Binop_i BOI_mul) ] ++
+    [ BI_global_get glob_tmp1 ; BI_global_get glob_tmp3 ; BI_binop T_i64 (Binop_i BOI_mul) ] ++
+    [ BI_global_get glob_tmp2 ; BI_global_get glob_tmp4 ; BI_binop T_i64 (Binop_i BOI_mul) ] ++
+    [ BI_global_get glob_tmp2 ; BI_global_get glob_tmp3 ; BI_binop T_i64 (Binop_i BOI_mul) ] ++
+    (* glob_tmp4 <- let lxy = lx * ly
             glob_tmp3 <- let lxhy = lx * hy
             glob_tmp2 <- let hxly = hx * ly
             glob_tmp1 <- let hxy  = hx * hy *)
-         [ BI_global_set glob_tmp4
-         ; BI_global_set glob_tmp3
-         ; BI_global_set glob_tmp2
-         ; BI_global_set glob_tmp1
-         ]  ++
-         (* glob_tmp4 <- let l = lxy | (hxy << 62) = glob_tmp4 | (glob_tmp1 << 62) *)
-         [ BI_global_get glob_tmp4
-         ; BI_global_get glob_tmp1
-         ; BI_const_num (nat_to_i64val 62)
-         ; BI_binop T_i64 (Binop_i BOI_shl)
-         ; BI_const_num maxuint63
-         ; BI_binop T_i64 (Binop_i BOI_and)
-         ; BI_binop T_i64 (Binop_i BOI_or)
-         ; BI_global_set glob_tmp4
-         ] ++
-         (* glob_tmp1 <- let h = hxy >> 1 = glob_tmp1 >> 1 *)
-         [ BI_global_get glob_tmp1
-         ; BI_const_num (nat_to_i64val 1)
-         ; BI_binop T_i64 (Binop_i (BOI_shr SX_U))
-         ; BI_global_set glob_tmp1
-         ] ++
-         (* glob_tmp3 <- let hl = hxly + lxhy = glob_tmp2 + glob_tmp3 *)
-         [ BI_global_get glob_tmp2
-         ; BI_global_get glob_tmp3
-         ; BI_binop T_i64 (Binop_i BOI_add)
-         ; BI_const_num maxuint63
-         ; BI_binop T_i64 (Binop_i BOI_and)
-         ; BI_global_set glob_tmp3
-         ] ++
-         (* glob_tmp1 <- let h = if hl < hxly then h + (1 << 31) else h *)
-         [ BI_global_get glob_tmp3
-         ; BI_global_get glob_tmp2
-         ; BI_relop T_i64 (Relop_i (ROI_lt SX_U))
-         ; BI_if (BT_valtype None)
-             [ BI_global_get glob_tmp1
-             ; BI_const_num (VAL_int64 (Wasm_int.Int64.repr 2147483648%Z))
-             ; BI_binop T_i64 (Binop_i BOI_add)
-             ; BI_global_set glob_tmp1
-             ]
-             [ ]
-         ] ++
-         (* glob_tmp2 <- let hl' = hl << 31 *)
-         [ BI_global_get glob_tmp3
-         ; BI_const_num (nat_to_i64val 31)
-         ; BI_binop T_i64 (Binop_i BOI_shl)
-         ; BI_const_num maxuint63
-         ; BI_binop T_i64 (Binop_i BOI_and)
-         ; BI_global_set glob_tmp2
-         ] ++
-         (* glob_tmp4 <- let l = l + hl' *)
-         [ BI_global_get glob_tmp4
-         ; BI_global_get glob_tmp2
-         ; BI_binop T_i64 (Binop_i BOI_add)
-         ; BI_const_num maxuint63
-         ; BI_binop T_i64 (Binop_i BOI_and)
-         ; BI_global_set glob_tmp4
-         ] ++
-         (* glob_tmp1 <- let h = if l < hl' then h + 1 else h *)
-         [ BI_global_get glob_tmp4
-         ; BI_global_get glob_tmp2
-         ; BI_relop T_i64 (Relop_i (ROI_lt SX_U))
-         ; BI_if (BT_valtype None)
-             [ BI_global_get glob_tmp1
-             ; BI_const_num (nat_to_i64val 1)
-             ; BI_binop T_i64 (Binop_i BOI_add)
-             ; BI_global_set glob_tmp1
-             ]
-             [ ]
-         ] ++
-         (* glob_tmp1 <- let h = h + (hl >> 32) *)
-         [ BI_global_get glob_tmp1
-         ; BI_global_get glob_tmp3
-         ; BI_const_num (nat_to_i64val 32)
-         ; BI_binop T_i64 (Binop_i (BOI_shr SX_U))
-         ; BI_binop T_i64 (Binop_i BOI_add)
-         ; BI_const_num maxuint63
-         ; BI_binop T_i64 (Binop_i BOI_and)
-         ; BI_global_set glob_tmp1
-         ] ++
-         load_local_i64 x ++
-         [ BI_const_num (nat_to_i64val 62)
-         ; BI_binop T_i64 (Binop_i (BOI_shr SX_U))
-         ; BI_testop T_i64 TO_eqz
-         ] ++
-         load_local_i64 y ++
-         [ BI_const_num (nat_to_i64val 62)
-         ; BI_binop T_i64 (Binop_i (BOI_shr SX_U))
-         ; BI_testop T_i64 TO_eqz
-         ; BI_binop T_i32 (Binop_i BOI_or)
-         ; BI_if (BT_valtype None)
-             [ ]
-             [ (* glob_tmp2 <- let l' := l + (x << 62) *)
-             BI_global_get glob_tmp4
-             ; BI_local_get x
-             ; BI_load T_i64 None 2%N 0%N
-             ; BI_const_num (nat_to_i64val 62)
-             ; BI_binop T_i64 (Binop_i BOI_shl)
-             ; BI_binop T_i64 (Binop_i BOI_add)
-             ; BI_const_num maxuint63
-             ; BI_binop T_i64 (Binop_i BOI_and)
-             ; BI_global_set glob_tmp2
-             (* glob_tmp1 <- let h := if l' < l then h + 1 else h *)
-             ; BI_global_get glob_tmp2
-             ; BI_global_get glob_tmp4
-             ; BI_relop T_i64 (Relop_i (ROI_lt SX_U))
-             ; BI_if (BT_valtype None)
-                 [ BI_global_get glob_tmp1
-                 ; BI_const_num (nat_to_i64val 1)
-                 ; BI_binop T_i64 (Binop_i BOI_add)
-                 ; BI_global_set glob_tmp1
-                 ]
-                 [ ]
-             (* return (h + (x >> 1), l') *)
-             ; BI_global_get glob_tmp1
-             ; BI_local_get x
-             ; BI_load T_i64 None 2%N 0%N
-             ; BI_const_num (nat_to_i64val 1)
-             ; BI_binop T_i64 (Binop_i (BOI_shr SX_U))
-             ; BI_binop T_i64 (Binop_i BOI_add)
-             ; BI_const_num maxuint63
-             ; BI_binop T_i64 (Binop_i BOI_and)
-             ; BI_global_set glob_tmp1
-             ; BI_global_get glob_tmp2
-             ; BI_global_set glob_tmp4
-             ]
-         ] ++ make_product glob_tmp1 glob_tmp4)
+    [ BI_global_set glob_tmp4
+      ; BI_global_set glob_tmp3
+      ; BI_global_set glob_tmp2
+      ; BI_global_set glob_tmp1
+    ]  ++
+    (* glob_tmp4 <- let l = lxy | (hxy << 62) = glob_tmp4 | (glob_tmp1 << 62) *)
+    [ BI_global_get glob_tmp4
+      ; BI_global_get glob_tmp1
+      ; BI_const_num (nat_to_i64val 62)
+      ; BI_binop T_i64 (Binop_i BOI_shl)
+      ; BI_const_num maxuint63
+      ; BI_binop T_i64 (Binop_i BOI_and)
+      ; BI_binop T_i64 (Binop_i BOI_or)
+      ; BI_global_set glob_tmp4
+    ] ++
+    (* glob_tmp1 <- let h = hxy >> 1 = glob_tmp1 >> 1 *)
+    [ BI_global_get glob_tmp1
+      ; BI_const_num (nat_to_i64val 1)
+      ; BI_binop T_i64 (Binop_i (BOI_shr SX_U))
+      ; BI_global_set glob_tmp1
+    ] ++
+    (* glob_tmp3 <- let hl = hxly + lxhy = glob_tmp2 + glob_tmp3 *)
+    [ BI_global_get glob_tmp2
+      ; BI_global_get glob_tmp3
+      ; BI_binop T_i64 (Binop_i BOI_add)
+      ; BI_const_num maxuint63
+      ; BI_binop T_i64 (Binop_i BOI_and)
+      ; BI_global_set glob_tmp3
+    ] ++
+    (* glob_tmp1 <- let h = if hl < hxly then h + (1 << 31) else h *)
+    [ BI_global_get glob_tmp3
+      ; BI_global_get glob_tmp2
+      ; BI_relop T_i64 (Relop_i (ROI_lt SX_U))
+      ; BI_if (BT_valtype None)
+          [ BI_global_get glob_tmp1
+            ; BI_const_num (VAL_int64 (Wasm_int.Int64.repr 2147483648%Z))
+            ; BI_binop T_i64 (Binop_i BOI_add)
+            ; BI_global_set glob_tmp1
+          ]
+          [ ]
+    ] ++
+    (* glob_tmp2 <- let hl' = hl << 31 *)
+    [ BI_global_get glob_tmp3
+      ; BI_const_num (nat_to_i64val 31)
+      ; BI_binop T_i64 (Binop_i BOI_shl)
+      ; BI_const_num maxuint63
+      ; BI_binop T_i64 (Binop_i BOI_and)
+      ; BI_global_set glob_tmp2
+    ] ++
+    (* glob_tmp4 <- let l = l + hl' *)
+    [ BI_global_get glob_tmp4
+      ; BI_global_get glob_tmp2
+      ; BI_binop T_i64 (Binop_i BOI_add)
+      ; BI_const_num maxuint63
+      ; BI_binop T_i64 (Binop_i BOI_and)
+      ; BI_global_set glob_tmp4
+    ] ++
+    (* glob_tmp1 <- let h = if l < hl' then h + 1 else h *)
+    [ BI_global_get glob_tmp4
+      ; BI_global_get glob_tmp2
+      ; BI_relop T_i64 (Relop_i (ROI_lt SX_U))
+      ; BI_if (BT_valtype None)
+          [ BI_global_get glob_tmp1
+            ; BI_const_num (nat_to_i64val 1)
+            ; BI_binop T_i64 (Binop_i BOI_add)
+            ; BI_global_set glob_tmp1
+          ]
+          [ ]
+    ] ++
+    (* glob_tmp1 <- let h = h + (hl >> 32) *)
+    [ BI_global_get glob_tmp1
+      ; BI_global_get glob_tmp3
+      ; BI_const_num (nat_to_i64val 32)
+      ; BI_binop T_i64 (Binop_i (BOI_shr SX_U))
+      ; BI_binop T_i64 (Binop_i BOI_add)
+      ; BI_const_num maxuint63
+      ; BI_binop T_i64 (Binop_i BOI_and)
+      ; BI_global_set glob_tmp1
+    ] ++
+    load_local_i64 x ++
+    [ BI_const_num (nat_to_i64val 62)
+      ; BI_binop T_i64 (Binop_i (BOI_shr SX_U))
+      ; BI_testop T_i64 TO_eqz
+    ] ++
+    load_local_i64 y ++
+    [ BI_const_num (nat_to_i64val 62)
+      ; BI_binop T_i64 (Binop_i (BOI_shr SX_U))
+      ; BI_testop T_i64 TO_eqz
+      ; BI_binop T_i32 (Binop_i BOI_or)
+      ; BI_if (BT_valtype None)
+          [ ]
+          [ (* glob_tmp2 <- let l' := l + (x << 62) *)
+            BI_global_get glob_tmp4
+            ; BI_local_get x
+            ; BI_load T_i64 None 2%N 0%N
+            ; BI_const_num (nat_to_i64val 62)
+            ; BI_binop T_i64 (Binop_i BOI_shl)
+            ; BI_binop T_i64 (Binop_i BOI_add)
+            ; BI_const_num maxuint63
+            ; BI_binop T_i64 (Binop_i BOI_and)
+            ; BI_global_set glob_tmp2
+                            (* glob_tmp1 <- let h := if l' < l then h + 1 else h *)
+            ; BI_global_get glob_tmp2
+            ; BI_global_get glob_tmp4
+            ; BI_relop T_i64 (Relop_i (ROI_lt SX_U))
+            ; BI_if (BT_valtype None)
+                [ BI_global_get glob_tmp1
+                  ; BI_const_num (nat_to_i64val 1)
+                  ; BI_binop T_i64 (Binop_i BOI_add)
+                  ; BI_global_set glob_tmp1
+                ]
+                [ ]
+                (* return (h + (x >> 1), l') *)
+            ; BI_global_get glob_tmp1
+            ; BI_local_get x
+            ; BI_load T_i64 None 2%N 0%N
+            ; BI_const_num (nat_to_i64val 1)
+            ; BI_binop T_i64 (Binop_i (BOI_shr SX_U))
+            ; BI_binop T_i64 (Binop_i BOI_add)
+            ; BI_const_num maxuint63
+            ; BI_binop T_i64 (Binop_i BOI_and)
+            ; BI_global_set glob_tmp1
+            ; BI_global_get glob_tmp2
+            ; BI_global_set glob_tmp4
+          ]
+    ] ++ make_product glob_tmp1 glob_tmp4.
 
-  else if Kername.eqb op_name primInt63Diveucl then
-    Ret ([ BI_local_get x
-         ; BI_load T_i64 None 2%N 0%N
-         ; BI_testop T_i64 TO_eqz
-         ; BI_if (BT_valtype None)
-             [ BI_const_num (nat_to_i64val 0)
-             ; BI_global_set glob_tmp1
-             ; BI_const_num (nat_to_i64val 0)
-             ; BI_global_set glob_tmp2
-             ]
-             [ BI_local_get y
-             ; BI_load T_i64 None 2%N 0%N
-             ; BI_testop T_i64 TO_eqz
-             ; BI_if (BT_valtype None)
-                 [ BI_const_num (nat_to_i64val 0)
-                 ; BI_global_set glob_tmp1
-                 ; BI_local_get x
-                 ; BI_load T_i64 None 2%N 0%N
-                 ; BI_global_set glob_tmp2
-                 ]
-                 (load_local_i64 x ++
-                  load_local_i64 y ++
-                  [ BI_binop T_i64 (Binop_i (BOI_div SX_U)) ; BI_global_set glob_tmp1 ] ++
-                  load_local_i64 x ++
-                  load_local_i64 y ++
-                  [ BI_binop T_i64 (Binop_i (BOI_rem SX_U)) ; BI_global_set glob_tmp2 ])
-             ]
-         ] ++ make_product glob_tmp1 glob_tmp2)
-  else
-    Err ("Unknown primitive arithmetic operator: " ++ (Kernames.string_of_kername op_name))%bs.
+Definition diveucl_instrs (x y : localidx) : list basic_instruction :=
+  [ BI_local_get x
+    ; BI_load T_i64 None 2%N 0%N
+    ; BI_testop T_i64 TO_eqz
+    ; BI_if (BT_valtype None)
+        [ BI_const_num (nat_to_i64val 0)
+          ; BI_global_set glob_tmp1
+          ; BI_const_num (nat_to_i64val 0)
+          ; BI_global_set glob_tmp2
+        ]
+        [ BI_local_get y
+          ; BI_load T_i64 None 2%N 0%N
+          ; BI_testop T_i64 TO_eqz
+          ; BI_if (BT_valtype None)
+              [ BI_const_num (nat_to_i64val 0)
+                ; BI_global_set glob_tmp1
+                ; BI_local_get x
+                ; BI_load T_i64 None 2%N 0%N
+                ; BI_global_set glob_tmp2
+              ]
+              (load_local_i64 x ++
+                 load_local_i64 y ++
+                 [ BI_binop T_i64 (Binop_i (BOI_div SX_U)) ; BI_global_set glob_tmp1 ] ++
+                 load_local_i64 x ++
+                 load_local_i64 y ++
+                 [ BI_binop T_i64 (Binop_i (BOI_rem SX_U)) ; BI_global_set glob_tmp2 ])
+        ]
+  ] ++ make_product glob_tmp1 glob_tmp2.
 
-Definition translate_primitive_unary_op op_name x : error (list basic_instruction) :=
-  if Kername.eqb op_name primInt63Head0 then
-    (* head0 x computes the leading number of zeros in x
-           OBS: need to subtract 1 since we're dealing with 63-bit integers *)
-    Ret (BI_global_get global_mem_ptr ::
-         load_local_i64 x ++
-         [ BI_unop T_i64 (Unop_i UOI_clz)
-         ; BI_const_num (nat_to_i64val 1)
-         ; BI_binop T_i64 (Binop_i BOI_sub)
-         ; BI_store T_i64 None 2%N 0%N
-         ; BI_global_get global_mem_ptr
-         ] ++ increment_global_mem_ptr 8)
+Definition translate_primitive_binary_op op (x y : localidx) : error (list basic_instruction) :=  
+  match op with
+  | PrimInt63add       => Ret (apply_binop_and_store_i64 BOI_add x y true)
+  | PrimInt63sub       => Ret (apply_binop_and_store_i64 BOI_sub x y true)
+  | PrimInt63mul       => Ret (apply_binop_and_store_i64 BOI_mul x y true)
+  | PrimInt63div       => Ret (div_instrs x y)
+  | PrimInt63mod       => Ret (mod_instrs x y)
+  | PrimInt63lsl       => Ret (shift_instrs x y BOI_shl true)
+  | PrimInt63lsr       => Ret (shift_instrs x y (BOI_shr SX_U) false)
+  | PrimInt63land      => Ret (apply_binop_and_store_i64 BOI_and x y false)
+  | PrimInt63lor       => Ret (apply_binop_and_store_i64 BOI_or x y false)
+  | PrimInt63lxor      => Ret (apply_binop_and_store_i64 BOI_xor x y false)
+  | PrimInt63eqb       => Ret (make_boolean_valued_comparison x y ROI_eq)
+  | PrimInt63ltb       => Ret (make_boolean_valued_comparison x y (ROI_lt SX_U))
+  | PrimInt63leb       => Ret (make_boolean_valued_comparison x y (ROI_le SX_U))
+  | PrimInt63compare   => Ret (compare_instrs x y)
+  | PrimInt63addc      => Ret (apply_exact_add_operation x y false)
+  | PrimInt63addcarryc => Ret (apply_exact_add_operation x y true) 
+  | PrimInt63subc      => Ret (apply_exact_sub_operation x y false) 
+  | PrimInt63subcarryc => Ret (apply_exact_sub_operation x y true)
+  | PrimInt63mulc      => Ret (mulc_instrs x y)
+  | PrimInt63diveucl   => Ret (diveucl_instrs x y)
+  | _ => Err "Unknown primitive binary operator"
+  end.
 
-  else if Kername.eqb op_name primInt63Tail0 then
-    (* tail0 x computes the trailing number of zeros in x
-           OBS: if x is 0, then result is 63 (can't just use wasm ctz op) ) *)
-    Ret (BI_global_get global_mem_ptr ::
-         load_local_i64 x ++
-         [ BI_testop T_i64 TO_eqz
-         ; BI_if (BT_valtype (Some (T_num T_i64)))
-             [ BI_const_num (nat_to_i64val 63) ]
-             (load_local_i64 x ++ [ BI_unop T_i64 (Unop_i UOI_ctz) ])
-         ; BI_store T_i64 None 2%N 0%N
-         ; BI_global_get global_mem_ptr
-         ] ++ increment_global_mem_ptr 8)
-  else
-    Err ("Unknown primitive unary operator: " ++ (Kernames.string_of_kername op_name))%bs.
+(* head0 x computes the leading number of zeros in x
+   OBS: need to subtract 1 since we're dealing with 63-bit integers *)
+Definition head0_instrs (x : localidx) : list basic_instruction := 
+  BI_global_get global_mem_ptr ::
+    load_local_i64 x ++
+    [ BI_unop T_i64 (Unop_i UOI_clz)
+      ; BI_const_num (nat_to_i64val 1)
+      ; BI_binop T_i64 (Binop_i BOI_sub)
+      ; BI_store T_i64 None 2%N 0%N
+      ; BI_global_get global_mem_ptr
+    ] ++ increment_global_mem_ptr 8.
 
-Definition div21_loop_body :=
+(* tail0 x computes the trailing number of zeros in x
+   OBS: if x is 0, then result is 63 (can't just use wasm ctz op) ) *)
+Definition tail0_instrs (x : localidx) : list basic_instruction :=
+  BI_global_get global_mem_ptr ::
+    load_local_i64 x ++
+    [ BI_testop T_i64 TO_eqz
+      ; BI_if (BT_valtype (Some (T_num T_i64)))
+          [ BI_const_num (nat_to_i64val 63) ]
+          (load_local_i64 x ++ [ BI_unop T_i64 (Unop_i UOI_ctz) ])
+      ; BI_store T_i64 None 2%N 0%N
+      ; BI_global_get global_mem_ptr
+    ] ++ increment_global_mem_ptr 8.
+
+Definition translate_primitive_unary_op op (x : localidx) : error (list basic_instruction) :=
+  match op with
+  | PrimInt63head0 => Ret (head0_instrs x)
+  | PrimInt63tail0 => Ret (tail0_instrs x)
+  | _ => Err "Unknown primitive unary operator"
+  end.
+
+Definition diveucl_21_loop_body :=
   [ BI_global_get glob_tmp1
   ; BI_const_num (nat_to_i64val 1)
   ; BI_binop T_i64 (Binop_i BOI_shl)
@@ -557,64 +550,166 @@ Definition div21_loop_body :=
       [ ]
   ].
 
-Definition translate_primitive_ternary_op op_name x y z : error (list basic_instruction) :=
-  if Kername.eqb op_name primInt63Diveucl_21 then
-    Ret (load_local_i64 z ++
-         [ BI_const_num maxuint63
-         ; BI_binop T_i64 (Binop_i BOI_and)
-         ; BI_global_set glob_tmp4
-         ] ++
-         load_local_i64 x ++
-         [ BI_const_num maxuint63
-         ; BI_binop T_i64 (Binop_i BOI_and)
-         ; BI_global_set glob_tmp1
-         ] ++
-         [ BI_global_get glob_tmp4
-         ; BI_global_get glob_tmp1
-         ; BI_relop T_i64 (Relop_i (ROI_le SX_U))
-         ; BI_if (BT_valtype (Some (T_num T_i32)))
-             ([ BI_const_num (nat_to_i64val 0) ; BI_global_set glob_tmp1 ] ++ make_product glob_tmp1 glob_tmp1)
-             (load_local_i64 y ++
-              [ BI_global_set glob_tmp2
-              ; BI_const_num (nat_to_i64val 0)
-              ; BI_global_set glob_tmp3
-              ] ++ (List.flat_map (fun x => x) (List.repeat div21_loop_body 63)) ++
-              [ BI_global_get glob_tmp1
-              ; BI_const_num maxuint63
-              ; BI_binop T_i64 (Binop_i BOI_and)
-              ; BI_global_set glob_tmp1
-              ] ++ (make_product glob_tmp3 glob_tmp1))
-         ])
+Definition diveucl_21_instrs (xh xl y : localidx) : list basic_instruction :=
+  load_local_i64 y ++ [ BI_global_set glob_tmp4 ] ++
+    load_local_i64 xh ++ [ BI_global_set glob_tmp1 ] ++
+    [ BI_global_get glob_tmp4
+      ; BI_global_get glob_tmp1
+      ; BI_relop T_i64 (Relop_i (ROI_le SX_U))
+      ; BI_if (BT_valtype (Some (T_num T_i32)))
+          ([ BI_const_num (nat_to_i64val 0) ; BI_global_set glob_tmp1 ] ++ make_product glob_tmp1 glob_tmp1)
+          (load_local_i64 xl ++
+             [ BI_global_set glob_tmp2
+               ; BI_const_num (nat_to_i64val 0)
+               ; BI_global_set glob_tmp3
+             ] ++ (List.flat_map (fun x => x) (List.repeat diveucl_21_loop_body 63)) ++
+             [ BI_global_get glob_tmp1
+               ; BI_const_num maxuint63
+               ; BI_binop T_i64 (Binop_i BOI_and)
+               ; BI_global_set glob_tmp1
+             ] ++ (make_product glob_tmp3 glob_tmp1))
+    ].
 
-  else if Kername.eqb op_name primInt63Addmuldiv then
-    Ret (BI_global_get global_mem_ptr ::
-         load_local_i64 x ++
-         [ BI_const_num (nat_to_i64val 63)
-         ; BI_relop T_i64 (Relop_i (ROI_gt SX_U))
-         ; BI_if (BT_valtype (Some (T_num T_i64)))
-             [ BI_const_num (nat_to_i64val 0) ]
-             (* Compute x << z on the stack *)
-             (load_local_i64 y ++
-              load_local_i64 x ++
-              [ BI_binop T_i64 (Binop_i BOI_shl)
-              ; BI_const_num maxuint63
-              ; BI_binop T_i64 (Binop_i BOI_and)
-              ] ++
-              (* Put y on the stack *)
-              load_local_i64 z ++
-              (* Compute 63 - z on the stack *)
-              [ BI_const_num (nat_to_i64val 63) ] ++
-              load_local_i64 x ++
-              [ BI_binop T_i64 (Binop_i BOI_sub)
-              (* Compute y >> (63 - z) on the stack *)
-              ; BI_binop T_i64 (Binop_i (BOI_shr SX_U))
-              (* Finally, compute (x << z) | (y >> (63 - z)) on the stack *)
-              ; BI_binop T_i64 (Binop_i BOI_or)
-              ])
-         ; BI_store T_i64 None 2%N 0%N
-         ; BI_global_get global_mem_ptr
-         ] ++ increment_global_mem_ptr 8)
+
+Definition addmuldiv_instrs p x y :=
+  BI_global_get global_mem_ptr ::
+    load_local_i64 p ++
+    [ BI_const_num (nat_to_i64val 63)
+      ; BI_relop T_i64 (Relop_i (ROI_gt SX_U))
+      ; BI_if (BT_valtype (Some (T_num T_i64)))
+          [ BI_const_num (nat_to_i64val 0) ]
+          (* Compute x << p on the stack *)
+          (load_local_i64 x ++
+             load_local_i64 p ++
+             [ BI_binop T_i64 (Binop_i BOI_shl)
+               ; BI_const_num maxuint63
+               ; BI_binop T_i64 (Binop_i BOI_and)
+             ] ++
+             (* Put y on the stack *)
+             load_local_i64 y ++
+             (* Compute 63 - p on the stack *)
+             [ BI_const_num (nat_to_i64val 63) ] ++
+             load_local_i64 p ++
+             [ BI_binop T_i64 (Binop_i BOI_sub)
+             (* Compute y >> (63 - p) on the stack *)
+             ; BI_binop T_i64 (Binop_i (BOI_shr SX_U))
+             (* Finally, compute (x << p) | (y >> (63 - p)) on the stack *)
+             ; BI_binop T_i64 (Binop_i BOI_or)
+             ])
+      ; BI_store T_i64 None 2%N 0%N
+      ; BI_global_get global_mem_ptr
+    ] ++ increment_global_mem_ptr 8.
+
+Definition translate_primitive_ternary_op op (x y z : localidx) : error (list basic_instruction) :=
+  match op with
+  | PrimInt63diveucl_21 => Ret (diveucl_21_instrs x y z)
+  | PrimInt63addmuldiv  => Ret (addmuldiv_instrs x y z)
+  | _ => Err "Unknown primitive ternary operator"
+  end.
+
+
+
+Definition LambdaANF_primInt_arith_fun (f : int63 -> int63 -> int63) (x y : int63) := Vprim (primInt (f x y)).
+  
+Definition LambdaANF_primInt_bool_fun (f : int63 -> int63 -> bool) x y :=
+  if f x y then
+    Vconstr true_tag []
   else
-    Err ("Unknown primitive arithmetic operator: " ++ (Kernames.string_of_kername op_name))%bs.
+    Vconstr false_tag [].
 
-End PrimitiveOperators.
+Definition LambdaANF_primInt_compare_fun (f : int63 -> int63 -> comparison) x y :=
+  match f x y with
+  | Datatypes.Eq => Vconstr eq_tag []
+  | Datatypes.Lt => Vconstr lt_tag []
+  | Datatypes.Gt => Vconstr gt_tag []
+  end.
+
+Definition LambdaANF_primInt_carry_fun (f : int63 -> int63 -> carry int63) x y :=
+  match f x y with
+  | C0 z => Vconstr c0_tag [ Vprim (primInt z) ]
+  | C1 z => Vconstr c1_tag [ Vprim (primInt z) ]
+  end.
+
+Definition LambdaANF_primInt_prod_fun (f : int63 -> int63 -> prod int63 int63) x y :=
+  let p := f x y in
+  Vconstr pair_tag [ Vprim (primInt (fst p)) ; Vprim (primInt (snd p)) ].
+
+Definition LambdaANF_primInt_unop_fun (f : int63 -> int63) x := Vprim (primInt (f x)).
+  
+Definition LambdaANF_primInt_diveucl_21 xh xl y := 
+  let (q, r) := diveucl_21 xh xl y in
+  Vconstr pair_tag [ Vprim (primInt q) ; Vprim (primInt r) ].
+
+Definition LambdaANF_primInt_addmuldiv p x y := Vprim (primInt (addmuldiv p x y)).
+
+(* Definition map_op_to_coq_def (op : primop) := *)
+(*   match op with *)
+(*   | PrimInt63add => Uint63.add *)
+(*   | PrimInt63sub => Uint63.sub *)
+(*   | PrimInt63mul => Uint63.mul *)
+(*   | PrimInt63div => Uint63.div *)
+(*   | PrimInt63mod => Uint63.mod *)
+(*   | PrimInt63lsl => Uint63.lsl *)
+(*   | PrimInt63lsr => Uint63.lsr *)
+(*   | PrimInt63land => Uint63.land *)
+(*   | PrimInt63lor => Uint63.lor *)
+(*   | PrimInt63lxor => Uint63.lxor *)
+(*   | PrimInt63eqb => Uint63.eqb *)
+(*   | PrimInt63ltb => Uint63.ltb *)
+(*   | PrimInt63leb => Uint63.leb *)
+(*   | PrimInt63compare => Uint63.compare *)
+(*   | PrimInt63addc => Uint63.addc *)
+(*   | PrimInt63addcarryc => Uint63.addcarryc *)
+(*   | PrimInt63subc => Uint63.subc *)
+(*   | PrimInt63subcarryc => Uint63.subcarryc *)
+(*   | PrimInt63mulc => Uint63.mulc *)
+(*   | PrimInt63head0 => Uint63.head0 *)
+(*   | PrimInt63tail0 => tail0 *)
+(*   | PrimInt63diveucl => diveucl *)
+(*   | PrimInt63Diveucl_21 => diveucl_21 *)
+(*   | PrimInt63addmuldiv => addmuldiv *)
+(*   end. *)
+
+
+Definition apply_LambdaANF_primInt_operator op (vs : list val) : option val :=
+  match vs with
+  | [ Vprim (primInt x) ] =>
+      match op with
+      | PrimInt63head0 => Some (LambdaANF_primInt_unop_fun Uint63.head0 x)
+      | PrimInt63tail0 => Some (LambdaANF_primInt_unop_fun Uint63.tail0 x)
+      | _ => None
+      end
+  | [ Vprim ( (primInt x) ) ; Vprim ( (primInt y) ) ] =>
+      match op with
+      | PrimInt63add => Some (LambdaANF_primInt_arith_fun Uint63.add x y)
+      | PrimInt63sub => Some (LambdaANF_primInt_arith_fun Uint63.sub x y)
+      | PrimInt63mul => Some (LambdaANF_primInt_arith_fun Uint63.mul x y)
+      | PrimInt63div => Some (LambdaANF_primInt_arith_fun Uint63.div x y)
+      | PrimInt63mod => Some (LambdaANF_primInt_arith_fun Uint63.mod x y)
+      | PrimInt63lsl => Some (LambdaANF_primInt_arith_fun Uint63.lsl x y)
+      | PrimInt63lsr => Some (LambdaANF_primInt_arith_fun Uint63.lsr x y)
+      | PrimInt63land => Some (LambdaANF_primInt_arith_fun Uint63.land x y)
+      | PrimInt63lor => Some (LambdaANF_primInt_arith_fun Uint63.lor x y)
+      | PrimInt63lxor => Some (LambdaANF_primInt_arith_fun Uint63.lxor x y)
+      | PrimInt63eqb => Some (LambdaANF_primInt_bool_fun Uint63.eqb x y)
+      | PrimInt63ltb => Some (LambdaANF_primInt_bool_fun Uint63.ltb x y)
+      | PrimInt63leb => Some (LambdaANF_primInt_bool_fun Uint63.leb x y)
+      | PrimInt63compare => Some (LambdaANF_primInt_compare_fun Uint63.compare x y)
+      | PrimInt63addc => Some (LambdaANF_primInt_carry_fun Uint63.addc x y) 
+      | PrimInt63addcarryc => Some (LambdaANF_primInt_carry_fun Uint63.addcarryc x y) 
+      | PrimInt63subc => Some (LambdaANF_primInt_carry_fun Uint63.subc x y) 
+      | PrimInt63subcarryc => Some (LambdaANF_primInt_carry_fun Uint63.subcarryc x y) 
+      | PrimInt63mulc => Some (LambdaANF_primInt_prod_fun Uint63.mulc x y)
+      | PrimInt63diveucl => Some (LambdaANF_primInt_prod_fun Uint63.diveucl x y)
+      | _ => None
+      end
+  | [ Vprim (primInt x) ; Vprim (primInt y) ; Vprim (primInt z) ] =>
+      match op with
+      | PrimInt63diveucl_21 => Some (LambdaANF_primInt_diveucl_21 x y z) 
+      | PrimInt63addmuldiv => Some (LambdaANF_primInt_addmuldiv x y z) 
+      | _ => None
+      end
+  | _ => None 
+  end.
+
+End Primitives.
